More theorems, including the useful w2i (i2w i) = i (as long as i is in the reasonable range)

src/integer/integer_wordScript.sml
@@ -1,6 +1,6 @@
 open HolKernel boolLib Parse bossLib BasicProvers
 
-open wordsTheory integerTheory
+open wordsTheory integerTheory intLib arithmeticTheory
 
 (* theory of 2's complement representation of integers *)
 
@@ -20,8 +20,11 @@ val UINT_MAX_def = Define`
 `;
 
 val INT_MAX_def = Define`
-  INT_MAX (x: 'a set) = 2n ** (dimindex (UNIV: 'a set) - 1) - 1
+  INT_MAX (x: 'a set) = 2i ** (dimindex (UNIV: 'a set) - 1) - 1
 `;
+val INT_MIN_def = Define`
+  INT_MIN x = ~INT_MAX x - 1
+`
 
 val INT_MAX_32 = store_thm(
   "INT_MAX_32",
@@ -29,44 +32,55 @@ val INT_MAX_32 = store_thm(
   SRW_TAC [][INT_MAX_def, dimindex_32]);
 val _ = export_rewrites ["INT_MAX_32"]
 
+val INT_MIN_32 = store_thm(
+  "INT_MIN_32",
+  ``INT_MIN (s: i32 set) = ~2147483648``,
+  SRW_TAC [][INT_MIN_def]);
+val _ = export_rewrites ["INT_MIN_32"]
+
 val UINT_MAX_32 = store_thm(
   "UINT_MAX_32",
   ``UINT_MAX (s: i32 set) = 4294967295``,
   SRW_TAC [][UINT_MAX_def, dimindex_32]);
 val _ = export_rewrites ["UINT_MAX_32"]
 
+val ONE_LE_TWOEXP = store_thm(
+  "ONE_LE_TWOEXP",
+  ``1n <= 2 ** m``,
+  SRW_TAC [][DECIDE ``1n <= x = 0 < x``]);
+val _ = export_rewrites ["ONE_LE_TWOEXP"]
+
 val w2i_n2w_pos = store_thm(
   "w2i_n2w_pos",
-  ``x <= INT_MAX (UNIV:'a set) ==>
-    (w2i (n2w x : bool ** 'a) = int_of_num x)``,
-  SRW_TAC [][w2i_def, word_msb_n2w, bitTheory.BIT_def,
+  ``&n <= INT_MAX (UNIV:'a set) ==>
+    (w2i (n2w n : bool ** 'a) = &n)``,
+  SRW_TAC [][w2i_def, word_msb_n2w, bitTheory.BIT_def, INT_SUB,
              bitTheory.BITS_def, DECIDE ``SUC x - x = 1``,
              bitTheory.DIV_2EXP_def, bitTheory.MOD_2EXP_def,
              w2n_n2w, INT_MAX_def, bitTheory.ZERO_LT_TWOEXP,
              DECIDE ``0n < y ==> (x <= y - 1 = x < y)``] THEN
-  FULL_SIMP_TAC (srw_ss()) [arithmeticTheory.LESS_DIV_EQ_ZERO] THEN
-  MATCH_MP_TAC arithmeticTheory.LESS_TRANS THEN
+  FULL_SIMP_TAC (srw_ss()) [LESS_DIV_EQ_ZERO] THEN
+  MATCH_MP_TAC LESS_TRANS THEN
   Q.EXISTS_TAC `2 ** (dimindex (UNIV:'a set) - 1)` THEN
   SRW_TAC [ARITH_ss][DIMINDEX_GT_0, bitTheory.TWOEXP_MONO]);
 
 val w2i_n2w_neg = store_thm(
   "w2i_n2w_neg",
-  ``INT_MAX (UNIV: 'a set) < x /\ x <= UINT_MAX (UNIV: 'a set) ==>
-      (w2i (n2w x : bool ** 'a) =
-          ~(2 ** dimindex (UNIV: 'a set) - int_of_num x))``,
-  SRW_TAC [][w2i_def, word_msb_n2w, bitTheory.BIT_def,
+  ``INT_MAX (UNIV: 'a set) < &n /\ n <= UINT_MAX (UNIV: 'a set) ==>
+      (w2i (n2w n : bool ** 'a) =
+          ~(2 ** dimindex (UNIV: 'a set) - &n))``,
+  SRW_TAC [][w2i_def, word_msb_n2w, bitTheory.BIT_def, INT_SUB,
              bitTheory.BITS_def, DECIDE ``SUC x - x = 1``,
              bitTheory.DIV_2EXP_def, bitTheory.MOD_2EXP_def,
              w2n_n2w, word_2comp_n2w, INT_MAX_def, UINT_MAX_def,
-             bitTheory.ZERO_LT_TWOEXP,
              DECIDE ``0n < y ==> (x <= y - 1 = x < y)``]
   THENL [
     SRW_TAC [ARITH_ss][GSYM INT_SUB],
-    `x DIV 2 ** (dimindex (UNIV: 'a set) - 1) = 1`
-       by (MATCH_MP_TAC arithmeticTheory.DIV_UNIQUE THEN
-           Q.EXISTS_TAC `x - 2 ** (dimindex (UNIV: 'a set) - 1)` THEN
+    `n DIV 2 ** (dimindex (UNIV: 'a set) - 1) = 1`
+       by (MATCH_MP_TAC DIV_UNIQUE THEN
+           Q.EXISTS_TAC `n - 2 ** (dimindex (UNIV: 'a set) - 1)` THEN
            SRW_TAC [ARITH_ss][bitTheory.ZERO_LT_TWOEXP] THEN
-           SRW_TAC [][GSYM (CONJUNCT2 arithmeticTheory.EXP)] THEN
+           SRW_TAC [][GSYM (CONJUNCT2 EXP)] THEN
            Q_TAC SUFF_TAC `SUC (dimindex (UNIV: 'a set) - 1) =
                            dimindex (UNIV: 'a set)` THEN1 SRW_TAC [][] THEN
            Q_TAC SUFF_TAC `0 < dimindex (UNIV: 'a set)` THEN1 DECIDE_TAC THEN
@@ -78,13 +92,49 @@ val w2i_n2w_neg = store_thm(
 val i2w_w2i = store_thm(
   "i2w_w2i",
   ``i2w (w2i w) = w``,
-  SRW_TAC [][w2i_def, i2w_def, n2w_w2n, WORD_NEG_NEG] THEN
-  FULL_SIMP_TAC (srw_ss()) [w2n_eq_0, WORD_NEG_EQ_0, WORD_NEG_0,
-                            w2n_n2w, bitTheory.ZERO_LT_TWOEXP]);
+  SRW_TAC [][w2i_def, i2w_def, n2w_w2n] THEN
+  FULL_SIMP_TAC (srw_ss()) []);
 
 
+val w2i_i2w = store_thm(
+  "w2i_i2w",
+  ``INT_MIN (UNIV : 'a set) <= i /\
+    i <= INT_MAX (UNIV : 'a set)
+      ==>
+    (w2i (i2w i : bool ** 'a) = i)``,
+  SIMP_TAC (srw_ss()) [INT_MIN_def, INT_MAX_def] THEN
+  Q.ABBREV_TAC `WL = 2n ** dimindex (UNIV : 'a set)` THEN
+  Q.ABBREV_TAC `HB = 2n ** (dimindex (UNIV : 'a set) - 1)` THEN
+  `WL = 2 * HB`
+     by (SRW_TAC [][Abbr`WL`, Abbr`HB`] THEN
+         `0 < dimindex (UNIV : 'a set)` by SRW_TAC [][DIMINDEX_GT_0] THEN
+         `?m. dimindex (UNIV : 'a set) = SUC m` by intLib.ARITH_TAC THEN
+         SRW_TAC [][EXP]) THEN
+  `0 < WL` by SRW_TAC [][Abbr`WL`, DIMINDEX_GT_0] THEN
+  `1 <= HB /\ 1 <= WL` by SRW_TAC [][Abbr`WL`, Abbr`HB`] THEN
+  ASM_SIMP_TAC (srw_ss()) [w2i_def, i2w_def, WORD_NEG_NEG, word_2comp_n2w,
+                           INT_LE, INT_SUB, INT_LE_SUB_RADD,
+                           NOT_LESS_EQUAL] THEN
+  Cases_on `i < 0` THENL [
+    `?n. ~(n = 0) /\ (i = ~&n)`
+       by (Q.SPEC_THEN `i` STRIP_ASSUME_TAC INT_NUM_CASES THEN
+           FULL_SIMP_TAC (srw_ss()) []) THEN
+    ASM_SIMP_TAC (srw_ss()) [word_msb_n2w_numeric, word_2comp_n2w] THEN
+    STRIP_TAC THEN
+    `n MOD (2 * HB) = n` by (MATCH_MP_TAC MOD_UNIQUE THEN
+                             Q.EXISTS_TAC `0` THEN DECIDE_TAC) THEN
+    `2 * HB - n < 2 * HB` by DECIDE_TAC THEN
+    ASM_SIMP_TAC (srw_ss() ++ ARITH_ss) [LESS_MOD],
 
-
+    `?n. i = &n`
+       by (Q.SPEC_THEN `i` STRIP_ASSUME_TAC INT_NUM_CASES THEN
+           FULL_SIMP_TAC (srw_ss()) []) THEN
+    ASM_SIMP_TAC (srw_ss()) [word_msb_n2w_numeric, word_2comp_n2w] THEN
+    STRIP_TAC THEN
+    `n MOD (2 * HB) = n` by (MATCH_MP_TAC MOD_UNIQUE THEN
+                             Q.EXISTS_TAC `0` THEN DECIDE_TAC) THEN
+    ASM_SIMP_TAC (srw_ss() ++ ARITH_ss) []
+  ])
 
 val _ = export_theory()
 
